\section{Lecture 7: Connections}

\[
\begin{aligned}
  & \nabla_X f = Xf = (df)(X) \text{ but (not quite) } \\ 
  & X : C^{\infty}(M) \to C^{\infty}(M) \\ 
  & df : \Gamma(TM) \to C^{\infty}(M) \\
  & \nabla_X : C^{\infty}(M) \to C^{\infty}(M)
\end{aligned}
\]

\begin{tikzpicture}[decoration=snake]
  \matrix (m) [matrix of math nodes, row sep=2em, column sep=3em, minimum width=1em]
  {
\nabla_X :   C^{\infty}(M) & C^{\infty}(M)   \\
\nabla_X :  \begin{aligned} \quad  \\ TM^p \otimes T^*M^q \text{ i.e. }  \\  \binom{p}{q} \text{ tensor field }  \end{aligned}   &  \begin{aligned} \quad \\ TM^p \otimes T^*M^q \text{ i.e. }  \\ \binom{p}{q} \text{ tensor field } \end{aligned} \\  };
%  \path[-stealth]
  \path[->]
  (m-1-1) edge node [above] {$$} (m-1-2)
%  edge node [left] {$\text{ev}_0$} (m-2-2)
%  (m-1-1) edge node [left] {$\alpha$} (m-2-1)
  (m-2-1) edge node [below] {$$} (m-2-2);
%  edge node [below] {$\pi_M$} (m-2-2);
  \path[->] %,decorate={zigzag,amplitude=0.7pt, segment length=1.2mm, pre=lineto,pre length=4pt}]
  (m-1-1) edge node [left] {$\vdots$} (m-2-1)
  (m-1-2) edge node [left] {$\vdots$} (m-2-2);
\end{tikzpicture}


\subsection{Directional derivatives of tensor fields}

manifold with connection is quadruple $(M, \mathcal{O}, \mathcal{A}, \nabla)$ 

topology $\mathcal{O}$

atlas $\mathcal{A}$

Consider chart $(U,x) \in \mathcal{A}$

\begin{definition}
$\forall \, $ pair $(X, (p,q)-\text{tensor field}) \equiv (X, (p,q)-TF)$,

\textbf{connection} $\nabla$ on smooth manifold $(M,\mathcal{O},\mathcal{A})$ 

$\nabla: ( X, (p,q)-TF) \to (p,q)-TF$ s.t.

\begin{enumerate}
  \item[(i)] $\nabla_X f = Xf $
  \item[(ii)]  $\nabla_X(T+S) = \nabla_XT + \nabla_XS $ 
\item[(iii)] \[
\nabla_X(T(\omega,Y)) = (\nabla_XT)(\omega,T) + T(\nabla_X\omega, Y) + T(\omega, \nabla_XY)
\]
``Leibnitz'' rule.

As
\[
T\otimes S (\omega_{(1)}\dots \omega_{(p+r)} , Y_{(1)} \dots Y_{(q+s)}) = T(\omega_{(1)} \dots \omega_{(p)}, Y_{(1)} \dots Y_{(q)} ) \cdot S( \omega_{(p+1)} \dots \omega_{(p+r)} , Y_{(q+1)} \dots Y_{(q+s)})
\]
so 
\[
\nabla_X(T\otimes S) = (\nabla_XT)\otimes S + T\otimes \nabla_XS
\]


\item[(iv)] $\nabla_{fX+Z} T = f\nabla_X T + \nabla_Z T$
$C^{\infty}$-linear
\end{enumerate}
\end{definition}

\subsection{New structure on $(M,\mathcal{O},\mathcal{A})$ required to fix $\nabla$}


There are $(\text{dim}M)^3$ many $\Gamma^i_{ \, \, j k}$
\[
\begin{aligned}
&  \Gamma^i_{ \, \, jk} : U \to \mathbb{R} \\ 
&  p \mapsto \left( dx^i ( \nabla_{ \frac{ \partial}{ \partial x} } \frac{ \partial }{ \partial x^j } ) \right)(p)
\end{aligned}
\]

Now $\nabla_{ \frac{ \partial }{ \partial x^m}  }(dx^i) = ?$

\[
\begin{aligned}
  & \underbrace{ \nabla_{  \frac{ \partial }{ \partial x^m} } ( \underbrace{ dx^i \left( \frac{ \partial }{ \partial x^j } \right) }_{ \delta^i_{ \, \, j} } ) }_{ \rotatebox{90}{$\,=$} \quad \, \text{ (iii) } }  = \frac{ \partial }{ \partial x^m} ( \delta^i_{ \, \, j} ) = 0  \\
& = \left( \nabla_{ \frac{ \partial }{ \partial x^m} } dx^i \right)\left( \frac{ \partial }{ \partial x^j} \right) + dx^i (   \underbrace{ \nabla_{ \frac{ \partial }{ \partial x^m } } \frac{ \partial }{ \partial x^j } }_{ \Gamma^q_{ \, jm }\frac{ \partial }{ \partial x^q} }   ) = 0 \\
& \Longrightarrow \left( \nabla_{ \frac{ \partial }{ \partial x^m } } dx^i \right)\left( \frac{ \partial }{ \partial x^j } \right) = - \Gamma^i_{ jm} \\
& \nabla_{ \frac{ \partial }{ \partial x^m} } dx^i = -\Gamma^i_{ jm} dx^j 
\end{aligned}
\]


% \rotatebox{90}{$\,=$}

Hence

\[
\begin{aligned}
  & ( \nabla_X Y)^i = X(Y^i) + \Gamma^i_{j\underbrace{m}_{\text{ last entry goes in direction of $X$ }} } Y^j X^m \\
  & (\nabla_X \omega)_i = X(\omega_i) + - \Gamma^j_{im} \omega_j X^m
\end{aligned}
\]
Note that for the immediately above expression for $(\nabla_X Y)^i$, in the second term on the right hand side, $\Gamma_{jm}^i$ has the last entry at the bottom, $m$ going in the direction of $X$, so that it matches up with $X^m$. This is a good mnemonic to memorize the index positions of $\Gamma$. 

\underline{summary so far}:
\[
\begin{aligned}
  & ( \nabla_X Y)^i = X(Y^i) + \Gamma^i_{jm }  Y^j X^m \\
  & (\nabla_X \omega)_i = X(\omega_i) + - \Gamma^j_{im} \omega_j X^m
\end{aligned}
\]
similarly, by further application of Leibnitz

$T$ a $(1,2)$-TF (tensor field)

\[
\begin{aligned}
  (\nabla_X T)^i_{ \, \, jk } = X(T^i_{ \, \, jk} ) + \Gamma^i_{ \, \, s m } T^s_{ \, \, jk} X^m - \Gamma^s_{ \, \, jm} T^i_{ \, \, sk} X^m - \Gamma^s_{ \, \, km} T^i_{ \,\, js} X^m
\end{aligned}
\]

What is a Euclidean space: \\
$(M = \mathbb{R}^n, \mathcal{O}_{\text{st}}, \mathcal{A})$ smooth manifold. \\
Assume $(\mathbb{R}^n, \text{id}_{\mathbb{R}^n} ) \in \mathcal{A}$ and 
\[
(\Gamma^i_{(x)})_{jk} = dx^i \left( (\nabla_{\text{\underline{E}}})_{ \frac{ \partial }{ \partial x^k} } \frac{ \partial }{ \partial x^j} \right) \overset{!}{=} 0 
\]


\subsection{Change of $\Gamma$'s under change of chart}

$(U,x)$, $(V,y) \in \mathcal{A}$ and $U \cap V \neq \emptyset$

\[
\Gamma^i_{jk}(y) := dy^i \left( \nabla_{ \frac{ \partial}{ \partial y^k} } \frac{ \partial }{ \partial y^j} \right) = \frac{ \partial y^i}{ \partial x^q }dx^q \left( \nabla_{\frac{ \partial x^p}{ \partial y^k}  \frac{ \partial }{ \partial x^p} } \frac{ \partial x^s}{ \partial y^j} \frac{ \partial }{ \partial x^s } \right)
\]

Note $\nabla_{fX}$ is $C^{\infty}$-linear for $fX$

covector $dy^i$ is $C^{\infty}$-linear in its argument
\[
\begin{aligned}
\Longrightarrow \Gamma_{jk}^i(y) & = \frac{ \partial y^i}{ \partial x^q} dx^q \left( \frac{ \partial x^p}{ \partial y^k} \left[ \left( \nabla_{ \frac{ \partial }{ \partial x^p} } \frac{ \partial x^s}{ \partial y^j} \right) \frac{ \partial }{ \partial x^s} + \frac{ \partial x^s}{ \partial y^j} \left( \nabla_{ \frac{ \partial }{ \partial x^p } } \frac{ \partial }{ \partial x^s } \right)  \right] \right) = \\
& = \frac{ \partial y^i}{ \partial x^q} \frac{ \partial x^p }{ \partial y^k} \frac{ \partial }{ \partial x^p } \frac{ \partial x^s}{ \partial y^j } \delta^q_{ \, \, s} + \frac{ \partial y^i}{ \partial x^q} \frac{ \partial x^p }{ \partial y^k} \frac{ \partial x^s}{ \partial y^j} \Gamma^q_{sp}(x)
\end{aligned}
\]


\begin{equation}\label{Eq:WEHCG0703_changeofGamma}
\Gamma^i_{jk}(y) = \frac{ \partial y^i}{ \partial x^q} \frac{ \partial^2 x^q}{ \partial y^j \partial y^k} + \frac{ \partial y^i}{ \partial x^q } \frac{ \partial x^s }{ \partial y^j} \frac{ \partial x^p }{ \partial y^k} \Gamma^q_{sp}(x)
\end{equation}
Eq. (\ref{Eq:WEHCG0703_changeofGamma}) is the change of connection coefficient function under the change of chart $(U\cap V,x) \to (U\cap V,y)$


\subsection{Normal Coordinates}
