\section{Lecture 10: Metric Manifolds}

cf. \href{https://youtu.be/ONCZNwKswn4}{Lecture 10: Metric Manifolds (International Winter School on Gravity and Light 2015)}

We establish a structure on a smooth manifold that allows one to assign vectors in each tangent space a length (and an angle between vectors in the same tangent space).

From this structure, one can then define a notion of length of a curve. \\
Then we can look at shortest curves.

Requiring then that the shortest curves coincide with the straightest curves (wrt $\nabla$) will result in $\nabla$ being determined by the metric structure.  

\[
g  \overset{ \substack{ \text{straight} = \text{short} \\ T =0 }  }{ \rightsquigarrow }  \nabla \rightsquigarrow \text{Riem}
\]


\subsection{Metrics}

\begin{definition}
  A metric $g$ on a smooth manifold $(M,\mathcal{O}, \mathcal{A})$ is a $(0,2)$-tensor field satisfying
\begin{enumerate}
  \item[(i)] \underline{symmetry} $g(X,Y) = g(Y,X)$ \, $\forall \, X, Y$ vector fields
\item[(ii)] \underline{non-degeneracy}: the \underline{musical map} 
\[
\begin{aligned}
  \text{``flat''} \, \,  \flat : \Gamma(TM) & \to \Gamma(T^*M) \\ 
  X \mapsto \flat(X)
\end{aligned}
\]
\emph{where} \quad \,  $\begin{aligned} & \quad \quad \\ 
  & \flat(X)(Y):= g(X,Y) \\
  & \flat(X) \in \Gamma(T^*M) \end{aligned}$ \\
In thought bubble: $\flat(X) = g(X,\cdot)$

\dots is a $C^{\infty}$-isomorphism in other words, it is invertible.  


\end{enumerate}
\end{definition}

\underline{Remark}: $(\flat(X))_a$ \quad \, or \\
$X_a$ \\
$(\flat(X))_a := g_{am} X^m$

Thought bubble: $\flat^{-1} = \sharp$

$\flat^{-1}(\omega)^a := g^{am}\omega_m$ \\
$\flat^{-1}(\omega)^a := (g^{``-1''})^{am}\omega_m$
$\Longrightarrow $ not needed.  (all of this is not needed)

\begin{definition}
  The $(2,0)$-tensor field $g^{``-1''}$ with respect to a metric $g$ is the symmetric
\[
\begin{aligned}
  g^{``-1''} : \Gamma(T^*M) \times \Gamma(T^*M) \xrightarrow{ ~ } C^{\infty}(M) \\
  (\omega, \sigma) \mapsto \omega( \flat^{-1}(\sigma)) \quad \quad \, \flat^{-1}(\sigma) \in \Gamma(TM))
\end{aligned}
\]

\underline{chart}: $\begin{aligned} & \quad \\ 
  & g_{ab} = g_{ba} \\
  & (g^{-1})^{am} g_{mb} = \delta^a_b \end{aligned}$


\end{definition}

\underline{Example}: $(S^2, \mathcal{O}, \mathcal{A})$ \\ 
\phantom{example } chart $(\mathcal{U}, x)$

$\begin{aligned} 
 & \varphi \in (0,2\pi ) \\ 
  & \theta \in (0,\pi)\end{aligned}$

\underline{define} the metric
\[
g_{ij}(x^{-1}(\theta,\varphi)) = \left[ \begin{matrix} R^2 & 0 \\
    0 & R^2\sin^2{\theta} \end{matrix} \right]_{ij}
\]
$R \in \mathbb{R}^+$

``the metric of the \underline{round sphere of radius $R$}''

\subsection{Signature} 

Linear algebra: \quad \quad \, $ \begin{aligned} & A^a_{\,\,m}v^m = \lambda v^a & \quad \quad \quad \, \left( \begin{matrix} \lambda_1 & & 0 \\
    & \ddots & \\ 
    0 & & \lambda_n \end{matrix} \right) \\
  & g_{am} v^m = \lambda \cdot v^a ? \rightsquigarrow  & \quad \quad \quad \, \left( \begin{matrix} 
    1        &   &    &        &    &   &        & \\
    & \ddots &   &    &        &    &   &        & \\
    &        & 1 &    &        &    &   &        & \\
    &        &   & -1 &        &    &   &        & \\
    &        &   &    & \ddots &    &   &        & \\
    &        &   &    &        & -1 &   &        & \\
    &        &   &    &        &    & 0 &        & \\
    &        &   &    &        &    &   & \ddots & \\
    &        &   &    &        &    &   &        & 0 \end{matrix} \right)
\end{aligned}$

$(1,1)$ tensor has eigenvalues \\
$(0,2)$ has \underline{signature} $(p,q)$ (well-defined)

$\left. \begin{aligned}
  (+++) \\
  (++-) \\
  (+--) \\
  (---) \end{aligned} \right\rbrace$ $d+1$ if $p+q = \text{dim}V$


\begin{definition} A metric is called  \\
\textbf{Riemannian} if its signature is $(++ \dots +)$ \\
\textbf{Lorentzian} if $(+-\dots -)$ 
\end{definition}


\subsection{Length of a curve}

Let $\gamma$ be a smooth curve. \\
Then we know its veloctiy $v_{\gamma, \gamma(\lambda)}$ at each $\gamma(\lambda) \in M$.  

\begin{definition}
  On a Riemannian metric manifold $M, \mathcal{O},\mathcal{A},g)$, the \textbf{speed} of a curve at $\gamma(\lambda)$ is the number 
\[
(\sqrt{ g(v_{\gamma}, v_{\gamma}) })_{\gamma(\lambda)} = s(\lambda)
\]
\end{definition}

F. Schuller: ``I feel the need for speed.'' -Top Gun.  

(I feel the need for speed, then I feel the need for a metric)

\underline{Aside}: $[v^a] = \frac{1}{T}$ \\
\phantom{Aside:} $[g_{ab}] = L^2 $ \\
\phantom{Aside:} $[\sqrt{g_{ab}v^av^b}] = \sqrt{ \frac{L^2}{T^2}} = \frac{L}{T}$

\begin{definition}
  Let $\gamma:(0,1) \to M$ a smooth curve.  \\
Then the \textbf{length of $\gamma$} is the number 
\[
\mathbb{R} \ni L[\gamma] := \int_0^1 d\lambda s(\lambda) = \int_0^1 d\lambda \sqrt{ (g(v_{\gamma}, v_{\gamma}))_{\gamma(\lambda)}}
\]
\end{definition}

F. Schuller: ``velocity is more fundamental than speed, speed is more fundamental than length''

\underline{Example}: reconsider the round sphere of radius $R$

Consider its equator: \\
$\begin{aligned}
&  \theta(\lambda) := (x^1 \circ \gamma)(\lambda) = \frac{\pi}{2} \\ 
 & \varphi(\lambda) := (x^2 \circ \gamma)(\lambda) = 2\pi \lambda^3   
\end{aligned}$

$\begin{aligned}
  & \theta'(\lambda) = 0 \\
  & \varphi'(\lambda) = 6\pi\lambda^2 
\end{aligned}$

on the same chart $g_{ij} = \left[ \begin{matrix} R^2 & \\ 
    & R^2 \sin^2{\theta} \end{matrix} \right]$

F.Schuller: do everything in this chart
\[
\begin{gathered}
L[\gamma] = \int_0^1 d\lambda \sqrt{ g_{ij}(x^{-1}(\theta(\lambda) , \varphi(\lambda)))(x^i\circ \gamma)'(\lambda)(x^j\circ \gamma)'(\lambda) } = \int_0^1 d\lambda \sqrt{ R^2 \cdot 0 + R^2\sin^2{(\theta(\lambda))} 36 \pi^2 \lambda^4 } = \\
= 6\pi R \int_0^1 d\lambda \lambda^2 = 6\pi R [ \frac{1}{3} \lambda^3 ]^1_0 = 2\pi R
\end{gathered}
\]

\begin{theorem}
  $\gamma: (0,1) \to M$ and \\
$\sigma:(0,1) \to (0,1)$ smooth bijective and \underline{increasing} ``reparametrization''
\[
L[\gamma] = L[\gamma \circ \sigma]
\]
\end{theorem}
\begin{proof}
  $\Longrightarrow $ Tutorials
\end{proof}

\subsection{Geodesics}

\begin{definition}
  A curve $\gamma:(0,1) \to M$ is called a \textbf{geodesic} on a Riemannian manifold $(M,\mathcal{O}, \mathcal{A}, g)$ if its a \emph{stationary} curve with respect to a length functional $L$.  
\end{definition}

Thought bubble: in classical mechanics, deform the curve a little, $\epsilon$ times this deformation, to first order, it agrees with $L[\gamma]$

\begin{theorem}
  $\gamma$ geodesic iff it satisfies the Euler-Lagrange equations for the Lagrangian
\end{theorem}

\[
\begin{aligned}
\mathcal{L}:& TM \to \mathbb{R} \\
& X \mapsto \sqrt{g(X,X)} \end{aligned}
\]
In a chart, the Euler Lagrange equations take the form:
\[
 \left( \frac{ \partial \mathcal{L}}{  \partial \dot{x}^m } \right)^{\cdot} - \frac{ \partial \mathcal{L}}{ \partial x^m} = 0 
\]
F.Schuller: this is a chart dependent formulation

\underline{here}: 
\[
\mathcal{L}(\gamma^i , \dot{\gamma}^i ) = \sqrt{ g_{ij}(\gamma(\lambda)) \dot{\gamma}^i(\lambda) \dot{\gamma}^j(\lambda)}
\]

Euler-Lagrange equations:
\[
\begin{aligned}
  & \frac{ \partial \mathcal{L}}{ \partial \dot{\gamma}^m } = \frac{1}{ \sqrt{  \dots } } g_{mj}(\gamma(\lambda)) \dot{\gamma}^j(\lambda) \\ 
  & \left( \frac{ \partial \mathcal{L}}{ \partial \dot{\gamma}^m } \right)^{\cdot} = \left( \frac{1}{ \sqrt{ \dots } } \right)^{\cdot} g_{mj}(\gamma(\lambda)) \cdot \dot{\gamma}^j(\lambda) + \frac{1}{\sqrt{ \dots }} \left( g_{mj}(\gamma(\lambda)) \ddot{\gamma}^j(\lambda) + \dot{\gamma}^s(\partial_s g_{mj}) \dot{\gamma}^j(\lambda) \right)
\end{aligned}
\]
Thought bubble: reparametrize $g(\dot{\gamma}, \dot{\gamma})=1$ (it's a condition on my reparametrization)

By a clever choice of reparametrization $( \frac{1}{\sqrt{ \dots }} )^{\cdot} =0$

\[
\begin{gathered}
  \frac{ \partial \mathcal{L}}{ \partial \gamma^m} = \frac{1}{ 2\sqrt{ \dots }} \partial_m g_{ij}(\gamma(\lambda)) \dot{\gamma}^i(\lambda) \dot{\gamma}^j(\lambda)
\end{gathered}
\]
putting this together as Euler-Lagrange equations:
\[
\begin{gathered}
g_{mj} \ddot{\gamma}^j +   \partial_s g_{mj} \dot{\gamma}^s \dot{\gamma}^j - \frac{1}{2} \partial_m g_{ij} \dot{\gamma}^i \dot{\gamma}^j = 0 
\end{gathered}
\]
Multiply on both sides $(g^{-1})^{qm}$
\[
\begin{gathered}
\ddot{\gamma^q} + (g^{-1})^{qm}(\partial_i g_{mj} - \frac{1}{2} \partial_m g_{ij} ) \dot{\gamma}^i \dot{\gamma}^j = 0  \\ 
\boxed{ \ddot{\gamma^q} + (g^{-1})^{qm}\frac{1}{2} (\partial_i g_{mj} + \partial_j g_{mi} -  \partial_m g_{ij} ) \dot{\gamma}^i \dot{\gamma}^j = 0 }
\end{gathered}
\]
geodesic equation for $\gamma$ in a chart.  

\[
\boxed{ (g^{-1})^{qm}\frac{1}{2} (\partial_i g_{mj} + \partial_j g_{mi} -  \partial_m g_{ij} ) =: \Gamma^q_{ \,\, ij}(\gamma(\lambda))
}
\]

Thought bubble: $\left( \frac{ \partial \mathcal{L}}{ \partial \xi_x^{a+\text{dim}M } } \right)^{\cdot}_{\sigma(x)} - \left( \frac{ \partial \mathcal{L}}{ \partial xi^a_x } \right)_{\sigma(x)} = 0$

\begin{definition}
``Christoffel symbol''   ${\,}^{\text{L.C.}}\Gamma$ are the connection coefficient functions of the so-called Levi-Civita connection ${\,}^{\text{L.C.}}\nabla$
\end{definition}
We usually make this choice of $\nabla$ if $g$ is given.  

$(M,\mathcal{O}, \mathcal{A},g) \to (M,\mathcal{O}, \mathcal{A}, g, {\,}^{\text{L.C.}}\nabla)$

\underline{abstract way}: $\nabla g = 0$ and $T=0$ (torsion) \\
$\Longrightarrow \nabla = {\,}^{\text{L.C.}}\nabla$


\begin{definition}
\begin{enumerate}
\item[(a)]
  The Riemann-Christoffel curvature is defined by 
\[
R_{abcd} := g_{am}R^m_{\,\,bcd}
\]
\item[(b)] Ricci: $R_{ab} = R^m_{\,\,amb}$ \\
Thought bubble: with a metric, ${\,}^{\text{L.C.}}\nabla$
\item[(c)] (Ricci) scalar curvature:
\[
R = g^{ab} R_{ab}
\]
Thought bubble: ${\,}^{\text{L.C.}}\nabla$
\end{enumerate}
\end{definition}

\begin{definition}
 \underline{ Einstein curvature } $(M,\mathcal{O}, \mathcal{A},g)$
\[
G_{ab}:= R_{ab} - \frac{1}{2} g_{ab} R
\]
\end{definition}

\underline{Convention}: $g^{ab} := (g^{``-1''})^{ab}$

F. Schuller: these indices are not being pulled up, because what would you pull them up with

(student) Question: Does the Einstein curvature yield new information?

Answer: 
\[
\begin{gathered}
  g^{ab} G_{ab} = R_{ab} g^{ab} - \frac{1}{2} g_{ab} g^{ab} R = R - \delta^a_a R = R - \frac{1}{2} \text{dim}M \, R = (1- \frac{d}{2}) R
\end{gathered}
\]

